src/cbor/pulse/CBOR.Pulse.API.Base.fst
@@ -403,34 +403,6 @@ let array_iterator_get_length_t
       pure (U64.v res == List.Tot.length y)
     )
 
-inline_for_extraction
-let array_iterator_share_t
-  (#t': Type)
-  (iter: perm -> t' -> list cbor -> slprop)
-= (x: t') ->
-  (#p: perm) ->
-  (#y: Ghost.erased (list cbor)) ->
-  stt_ghost unit emp_inames
-    (iter p x y)
-    (fun _ ->
-      iter (p /. 2.0R) x y ** iter (p /. 2.0R) x y
-    )
-
-inline_for_extraction
-let array_iterator_gather_t
-  (#t': Type)
-  (iter: perm -> t' -> list cbor -> slprop)
-= (x: t') ->
-  (#p1: perm) ->
-  (#y1: Ghost.erased (list cbor)) ->
-  (#p2: perm) ->
-  (#y2: Ghost.erased (list cbor)) ->
-  stt_ghost unit emp_inames
-    (iter p1 x y1 ** iter p2 x y2)
-    (fun _ ->
-      iter (p1 +. p2) x y1 ** pure (y1 == y2)
-    )
-
 let get_map_length_post
   (y: cbor)
   (res: FStar.UInt64.t)
@@ -515,34 +487,6 @@ let map_iterator_next_t
     )
 
 inline_for_extraction
-let map_iterator_share_t
-  (#t': Type)
-  (iter: perm -> t' -> list (cbor & cbor) -> slprop)
-= (x: t') ->
-  (#p: perm) ->
-  (#y: Ghost.erased (list (cbor & cbor))) ->
-  stt_ghost unit emp_inames
-    (iter p x y)
-    (fun _ ->
-      iter (p /. 2.0R) x y ** iter (p /. 2.0R) x y
-    )
-
-inline_for_extraction
-let map_iterator_gather_t
-  (#t': Type)
-  (iter: perm -> t' -> list (cbor & cbor) -> slprop)
-= (x: t') ->
-  (#p1: perm) ->
-  (#y1: Ghost.erased (list (cbor & cbor))) ->
-  (#p2: perm) ->
-  (#y2: Ghost.erased (list (cbor & cbor))) ->
-  stt_ghost unit emp_inames
-    (iter p1 x y1 ** iter p2 x y2)
-    (fun _ ->
-      iter (p1 +. p2) x y1 ** pure (y1 == y2)
-    )
-
-inline_for_extraction
 let map_entry_key_t
   (#t2 #t: Type)
   (vmatch2: perm -> t2 -> cbor & cbor -> slprop)
@@ -574,6 +518,7 @@ let map_entry_value_t
 
 (** Permissions *)
 
+inline_for_extraction
 let share_t
   (#t1 #t2: Type)
   (vmatch: perm -> t1 -> t2 -> slprop)
@@ -588,6 +533,7 @@ let share_t
     vmatch (p /. 2.0R) x1 x2 ** vmatch (p /. 2.0R) x1 x2
   )
 
+inline_for_extraction
 let gather_t
   (#t1 #t2: Type)
   (vmatch: perm -> t1 -> t2 -> slprop)
